

Given (for all proofs below)

$V = IR + E_{mf}$ by Ohm's Law with back EMF for a DC motor

$E_{mf} = \omega\kappa_e$ by the Back EMF equation of a motor

$\tau = I\kappa_t$ by the Motor torque equation

$\tau = J\alpha + B\omega + \tau_{load} \text{sign}(\omega)$ by the Rotational equation of motion

The value of ω and α (Only for the proof directly below this)

Find V voltage

$V = IR + E_{mf}$, $E_{mf} = \omega\kappa_e$, $\tau = I\kappa_t$, $\tau = J\alpha + B\omega + \tau_{load} \text{sign}(\omega)$, and the value of ω and α because they are given

$I\kappa_t = J\alpha + B\omega + \tau_{load} \text{sign}(\omega)$ By substitution

$I = \frac{J\alpha + B\omega + \tau_{load} \text{sign}(\omega)}{\kappa_t}$ By Division

$-IR = E_{mf} - V$ By Subtraction

$I = \frac{E_{mf} - V}{-R}$ By Division

$\frac{E_{mf} - V}{-R} = \frac{J\alpha + B\omega + \tau_{load} \text{sign}(\omega)}{\kappa_t}$ By substitution

$\frac{\omega\kappa_e - V}{-R} = \frac{J\alpha + B\omega + \tau_{load} \text{sign}(\omega)}{\kappa_t}$ By substitution

$\omega\kappa_e - V = \frac{J\alpha + B\omega + \tau_{load} \text{sign}(\omega)}{\kappa_t}(-R)$ By multiplication

$-V = \frac{J\alpha + B\omega + \tau_{load} \text{sign}(\omega)}{\kappa_t}(-R) - \omega\kappa_e$ By subtraction

$V = -\left(\frac{J\alpha + B\omega + \tau_{load} \text{sign}(\omega)}{\kappa_t}(-R) - \omega\kappa_e\right)$ By division

$V = \frac{J\alpha + B\omega + \tau_{load} \text{sign}(\omega)}{\kappa_t}(R) + \omega\kappa_e$ By substitution

$V = \frac{J\alpha R}{\kappa_t} + \frac{B\omega R}{\kappa_t} + \frac{\tau_{load} \text{sign}(\omega)R}{\kappa_t} + \frac{\omega\kappa_e\kappa_t}{\kappa_t}$ By substitution

$V = \frac{J\alpha R}{\kappa_t} + \frac{B\omega R + \omega\kappa_e\kappa_t}{\kappa_t} + \frac{\tau_{load} \text{sign}(\omega)R}{\kappa_t}$ By substitution

$V = \frac{J\alpha R}{\kappa_t} + \frac{\omega(BR + \kappa_e\kappa_t)}{\kappa_t} + \frac{\tau_{load} \text{sign}(\omega)R}{\kappa_t}$ By substitution

Define K_v by $K_v = \frac{BR + \kappa_e\kappa_t}{\kappa_t}$

Define K_a by $K_a = \frac{JR}{\kappa_t}$

Define K_s by $K_s = \frac{\tau_{load} R}{\kappa_t}$

$V = K_a\alpha + K_v\omega + K_s \text{sign}(\omega)$

Define a function V by $V(\omega, \alpha) = K_a\alpha + K_v\omega + K_s \text{sign}(\omega)$

■

Given (Only for the proof directly below this)

The value of ω

Find the maximum α angular acceleration at some angular velocity ω

$V = IR + E_{mf}$, $E_{mf} = \omega\kappa_e$, $\tau = I\kappa_t$, $\tau = J\alpha + B\omega + \tau_{load} \text{sign}(\omega)$, and the value of ω because they are given

Note: The VEX motor controller has current limits so we must also account for those.

Define I_{\min} and I_{\max} as the current limits and define I_{clamp} as the clamped value of I

Define V_{\max} as the maximum voltage and set it to V when finding the max acceleration

Define α_{\max} as the maximum voltage and set it to α when finding the max acceleration

$I_{\text{clamp}} = \min(\max(I, I_{\min}), I_{\max})$ by the definition of clamping

$I_{\text{clamp}} = \min(\max(\left(\frac{E_{\text{mf}} - V_{\max}}{-R}\right), I_{\min}), I_{\max})$ by substitution

$I_{\text{clamp}} = \min(\max(\left(\frac{\omega \kappa_e - V_{\max}}{-R}\right), I_{\min}), I_{\max})$ by substitution

Define $V_{\max} = V$ as the max voltage

$I_{\text{clamp}} = \min(\max(\left(\frac{\omega \kappa_e - V_{\max}}{-R}\right), I_{\min}), I_{\max})$ by substitution

Restrict I by $I_{\text{clamp}} = I$ by the note

$-J\alpha_{\max} = B\omega + \tau_{\text{load}} \text{sign}(\omega) - \tau$ by Subtraction

$\alpha_{\max} = \frac{B\omega + \tau_{\text{load}} \text{sign}(\omega) - \tau}{-J}$ by Division

$\alpha_{\max} = \frac{B\omega + \tau_{\text{load}} \text{sign}(\omega) - I\kappa_t}{-J}$ by Substitution

$\alpha_{\max} = \frac{B\omega + \tau_{\text{load}} \text{sign}(\omega) - I_{\text{clamp}}\kappa_t}{-J}$ by Substitution

Define a function α by $\alpha_{\max}(\omega) = \frac{B\omega + \tau_{\text{load}} \text{sign}(\omega) - I_{\text{clamp}}\kappa_t}{-J}$

■

Find $\omega(t)$ given that the motor is constantly accelerating

$$\alpha_{\max}(\omega) = \frac{V_{\max} - K_v\omega - \text{sgn}(\omega)K_s}{K_a}$$

Let $s = \text{sgn}(\omega) \in \{1, -1\}$

$$\frac{d\omega}{dt} = \frac{V_{\max} - K_v\omega - sK_s}{K_a}$$

$$\frac{d\omega}{dt} + \frac{K_v}{K_a}\omega = \frac{V_{\max} - sK_s}{K_a}$$

$$I(t) = e^{\int \frac{K_v}{K_a} dt}$$

$$I(t) = e^{\frac{K_v}{K_a} t}$$

$$\omega(t) = \frac{1}{I(t)} \left(\int_0^t I(\tau) Q d\tau + I(0)\omega_0 \right)$$

$$\omega(t) = \frac{1}{e^{\frac{K_v}{K_a} t}} \left(\int_0^t e^{\frac{K_v}{K_a} \tau} \frac{V_{\max} - sK_s}{K_a} d\tau + \omega_0 \right)$$

$$\omega(t) = \frac{1}{e^{\frac{K_v}{K_a} t}} \left(\frac{V_{\max} - sK_s}{K_a} \frac{K_a}{K_v} \left(e^{\frac{K_v}{K_a} \tau} - 1 \right) + \omega_0 \right)$$

$$\omega(t) = \frac{V_{\max} - sK_s}{K_v} \frac{e^{\frac{K_v}{K_a} \tau} - 1}{e^{\frac{K_v}{K_a} t}} + \omega_0 \left(e^{-\frac{K_v}{K_a} t} \right)$$

$$\omega(t) = \frac{V_{\max} - sK_s}{K_v} + \left(\omega_0 - \frac{V_{\max} - sK_s}{K_v} \right) e^{-\frac{K_v}{K_a} t}$$

■

Find a State-Space model in the form

$$\dot{x} = Ax + Bu$$

$$y = Cx + Du$$

$V = K_a\alpha + K_v\omega + K_s \text{sign}(\omega)$ because it is given

Let $u = V$ and $x = \begin{pmatrix} \omega \\ \text{sign}(\omega) \end{pmatrix}$

$\alpha = \dot{\omega}$ by the definition of acceleration

$\dot{x}(1 \ 0) = \dot{\omega}$ by the derivative

$\alpha = \dot{x}(1 \ 0)$ by substitution

$\text{sign}(\omega) = x(0 \ 1)$

$u = K_a \alpha + K_v \omega + K_s \text{sign}(\omega)$ by substitution

$K_v \omega + K_s \text{sign}(\omega) = -K_a \alpha + u$ by subtraction

$K_v x(1 \ 0) + K_s x(0 \ 1) = -K_a \dot{x}(1 \ 0) + u$ by substitution

$x(K_v(1 \ 0) + K_s(0 \ 1)) = -K_a \dot{x}(1 \ 0) + u$ by substitution

$x(K_v \ K_s) = -K_a \dot{x}(1 \ 0) + u$ by substitution

$x = (K_v \ K_s)^+ (-K_a \dot{x}(1 \ 0) + u)$ by multiplication

$x = \frac{\begin{pmatrix} K_v \\ K_s \end{pmatrix}}{K_v^2 + K_s^2} (-K_a \dot{x}(1 \ 0) + u)$ by the psuedoinverse

$x = -\frac{K_a}{K_v^2 + K_s^2} \begin{pmatrix} K_v & 0 \\ K_s & 0 \end{pmatrix} \dot{x} + \frac{1}{K_v^2 + K_s^2} \begin{pmatrix} K_v \\ K_s \end{pmatrix} u$ by substitution

$x = \begin{pmatrix} \frac{-K_a K_v}{K_v^2 + K_s^2} & 0 \\ \frac{-K_a K_s}{K_v^2 + K_s^2} & 0 \end{pmatrix} \dot{x} + \begin{pmatrix} \frac{-K_a K_v}{K_v^2 + K_s^2} \\ \frac{-K_a K_s}{K_v^2 + K_s^2} \end{pmatrix} u$ by substitution

■